Closure.thy
@@ -42,6 +42,31 @@ qed
 
 section \<open>Old Variant Using a Global Set of Regions\<close>
 
+paragraph \<open>Shared Definitions for Local and Global Sets of Regions\<close>
+
+locale Alpha_defs =
+  fixes X :: "'c set"
+begin
+
+definition V :: "('c, t) cval set" where "V \<equiv> {v . \<forall> x \<in> X. v x \<ge> 0}"
+
+lemma up_V: "Z \<subseteq> V \<Longrightarrow> Z\<^sup>\<up> \<subseteq> V"
+unfolding V_def zone_delay_def cval_add_def by auto
+
+lemma reset_V: "Z \<subseteq> V \<Longrightarrow> (zone_set Z r) \<subseteq> V"
+unfolding V_def unfolding zone_set_def by (induction r, auto)
+
+lemma step_z_V: "A \<turnstile> \<langle>l, Z\<rangle> \<leadsto>\<^bsub>a\<^esub> \<langle>l',Z'\<rangle> \<Longrightarrow> Z \<subseteq> V \<Longrightarrow> Z' \<subseteq> V"
+ apply (induction rule: step_z.induct)
+  apply (rule le_infI1)
+  apply (rule up_V)
+  apply blast
+ apply (rule le_infI1)
+ apply (rule reset_V)
+by blast
+
+end
+
 text \<open>
   This is the classic variant using a global clock ceiling \<open>k\<close> and thus a global set of regions.
   It is also the version that is necessary to prove the classic extrapolation correct.
@@ -49,10 +74,10 @@ text \<open>
   adoptions that are necessary to obtain the new version.
 \<close>
 
-locale AlphaClosure_old =
-  fixes X k \<R> and V :: "('c, t) cval set"
+locale AlphaClosure_global =
+  Alpha_defs X for X :: "'c set" +
+  fixes k \<R>
   defines "\<R> \<equiv> {region X I r | I r. valid_region X k I r}"
-  defines "V \<equiv> {v . \<forall> x \<in> X. v x \<ge> 0}"
   assumes finite: "finite X"
 begin
 
@@ -69,7 +94,6 @@ by auto (drule valid_regions_distinct, assumption+, simp)+
 definition cla ("Closure\<^sub>\<alpha> _" [71] 71)
 where
   "cla Z = \<Union> {R \<in> \<R>. R \<inter> Z \<noteq> {}}"
-
 
 subsubsection \<open>The Nice and Easy Properties Proved by Bouyer\<close>
 
@@ -258,22 +282,6 @@ where
 inductive_cases[elim!]: "A \<turnstile> \<langle>l, u\<rangle> \<leadsto>\<^bsub>\<alpha>(a)\<^esub> \<langle>l',u'\<rangle>"
 
 declare step_z_alpha.intros[intro]
-
-lemma up_V: "Z \<subseteq> V \<Longrightarrow> Z\<^sup>\<up> \<subseteq> V"
-unfolding V_def zone_delay_def cval_add_def by auto
-
-lemma reset_V: "Z \<subseteq> V \<Longrightarrow> (zone_set Z r) \<subseteq> V"
-unfolding V_def unfolding zone_set_def by (induction r, auto)
-
-lemma step_z_V: "A \<turnstile> \<langle>l, Z\<rangle> \<leadsto>\<^bsub>a\<^esub> \<langle>l',Z'\<rangle> \<Longrightarrow> Z \<subseteq> V \<Longrightarrow> Z' \<subseteq> V"
- apply (induction rule: step_z.induct)
-  apply (rule le_infI1)
-  apply (rule up_V)
-  apply blast
- apply (rule le_infI1)
- apply (rule reset_V)
-by blast
-
 
 text \<open>Single-step soundness and completeness follows trivially from \<open>cla_empty_iff\<close>.\<close>
 
@@ -740,9 +748,9 @@ where
   \<Longrightarrow> valid_abstraction A X k"
 
 locale AlphaClosure =
-  fixes X and k :: "'s \<Rightarrow> 'c \<Rightarrow> nat" and \<R> and V :: "('c, t) cval set"
+  Alpha_defs X for X :: "'c set" +
+  fixes k :: "'s \<Rightarrow> 'c \<Rightarrow> nat" and \<R>
   defines "\<R> l \<equiv> {region X I r | I r. valid_region X (k l) I r}"
-  defines "V \<equiv> {v . \<forall> x \<in> X. v x \<ge> 0}"
   assumes finite: "finite X"
 begin
 
@@ -750,196 +758,6 @@ definition cla ("Closure\<^sub>\<alpha>\<^sub>,\<^sub>_(_)" [71,71] 71)
 where
   "cla l Z = \<Union> {R \<in> \<R> l. R \<inter> Z \<noteq> {}}"
 
-context
-  fixes l :: 's
-begin
-
-lemmas set_of_regions_spec = set_of_regions[OF _ _ _ finite, of _ "k l", folded \<R>_def]
-lemmas region_cover_spec = region_cover[of X _ "k l", folded \<R>_def]
-lemmas region_unique_spec = region_unique[of "\<R> l" X "k l", folded \<R>_def, simplified]
-lemmas regions_closed'_spec = regions_closed'[of "\<R> l" X "k l", folded \<R>_def, simplified]
-
-lemma valid_regions_distinct_spec:
-  "R \<in> \<R> l \<Longrightarrow> R' \<in> \<R> l \<Longrightarrow> v \<in> R \<Longrightarrow> v \<in> R' \<Longrightarrow> R = R'"
-unfolding \<R>_def using valid_regions_distinct
-  by auto (drule valid_regions_distinct, assumption+, simp)+
-
-
-subsubsection \<open>The Nice and Easy Properties Proved by Bouyer\<close>
-
-lemma closure_constraint_id:
-  "\<forall>(x, m)\<in>collect_clock_pairs g. m \<le> real (k l x) \<and> x \<in> X \<and> m \<in> \<nat> \<Longrightarrow> Closure\<^sub>\<alpha>\<^sub>,\<^sub>l(\<lbrace>g\<rbrace>) = \<lbrace>g\<rbrace> \<inter> V"
-proof goal_cases
-  case 1
-  show ?case
-  proof auto
-    fix v assume v: "v \<in> Closure\<^sub>\<alpha>\<^sub>,\<^sub>l \<lbrace>g\<rbrace>"
-    then obtain R where R: "v \<in> R" "R \<in> \<R> l" "R \<inter> \<lbrace>g\<rbrace> \<noteq> {}" unfolding cla_def by auto
-    with ccompatible[OF 1, folded \<R>_def] show "v \<in> \<lbrace>g\<rbrace>" unfolding ccompatible_def by auto
-    from R show "v \<in> V" unfolding V_def \<R>_def by auto
-  next
-    fix v assume v: "v \<in> \<lbrace>g\<rbrace>" "v \<in> V"
-    with region_cover[of X v "k l", folded \<R>_def] obtain R where "R \<in> \<R> l" "v \<in> R"
-      unfolding V_def by auto
-    then show "v \<in> Closure\<^sub>\<alpha>\<^sub>,\<^sub>l \<lbrace>g\<rbrace>" unfolding cla_def using v by auto
-  qed
-qed
-
-lemma closure_id':
-  "Z \<noteq> {} \<Longrightarrow> Z \<subseteq> R \<Longrightarrow> R \<in> \<R> l \<Longrightarrow> Closure\<^sub>\<alpha>\<^sub>,\<^sub>l Z = R"
-proof goal_cases
-  case 1
-  note A = this
-  then have "R \<subseteq> Closure\<^sub>\<alpha>\<^sub>,\<^sub>l Z" unfolding cla_def by auto
-  moreover
-  { fix R' assume R': "Z \<inter> R' \<noteq> {}" "R' \<in> \<R> l" "R \<noteq> R'"
-    with A obtain v where "v \<in> R" "v \<in> R'" by auto
-    with \<R>_regions_distinct[OF _ A(3) this(1) R'(2-)] \<R>_def have False by auto
-  }
-  ultimately show ?thesis unfolding cla_def by auto
-qed
-
-lemma closure_id:
-  "Closure\<^sub>\<alpha>\<^sub>,\<^sub>l Z \<noteq> {} \<Longrightarrow> Z \<subseteq> R \<Longrightarrow> R \<in> \<R> l \<Longrightarrow> Closure\<^sub>\<alpha>\<^sub>,\<^sub>l Z = R"
-proof goal_cases
-  case 1
-  then have "Z \<noteq> {}" unfolding cla_def by auto
-  with 1 closure_id' show ?case by blast
-qed
-
-lemma closure_update_mono:
-  "Z \<subseteq> V \<Longrightarrow> set r \<subseteq> X \<Longrightarrow> zone_set (Closure\<^sub>\<alpha>\<^sub>,\<^sub>l Z) r \<subseteq> Closure\<^sub>\<alpha>\<^sub>,\<^sub>l(zone_set Z r)"
-proof -
-  assume A: "Z \<subseteq> V" "set r \<subseteq> X"
-  let ?U = "{R \<in> \<R> l. Z \<inter> R \<noteq> {}}"
-  from A(1) region_cover_spec  have "\<forall> v \<in> Z. \<exists> R. R \<in> \<R> l \<and> v \<in> R" unfolding V_def by auto
-  then have "Z = \<Union> {Z \<inter> R | R. R \<in> ?U}"
-  proof (auto, goal_cases)
-    case (1 v)
-    then obtain R where "R \<in> \<R> l" "v \<in> R" by auto
-    moreover with 1 have "Z \<inter> R \<noteq> {}" "v \<in> Z \<inter> R" by auto
-    ultimately show ?case by auto
-  qed
-  then obtain U where U: "Z = \<Union> {Z \<inter> R | R. R \<in> U}" "\<forall> R \<in> U. R \<in> \<R> l" by blast
-  { fix R assume R: "R \<in> U"
-    { fix v' assume v': "v' \<in> zone_set (Closure\<^sub>\<alpha>\<^sub>,\<^sub>l (Z \<inter> R)) r - Closure\<^sub>\<alpha>\<^sub>,\<^sub>l(zone_set (Z \<inter> R) r)"
-      then obtain v where *:
-        "v \<in> Closure\<^sub>\<alpha>\<^sub>,\<^sub>l(Z \<inter> R)" "v' = [r \<rightarrow> 0]v"
-      unfolding zone_set_def by auto
-      with closure_id[of "Z \<inter> R" R] R U(2) have **:
-        "Closure\<^sub>\<alpha>\<^sub>,\<^sub>l(Z \<inter> R) = R" "Closure\<^sub>\<alpha>\<^sub>,\<^sub>l(Z \<inter> R) \<in> \<R> l"
-      by fastforce+
-      with region_set'_id[OF _ *(1) finite _ _ A(2), of "k l" 0, folded \<R>_def, OF this(2)]
-      have ***: "zone_set R r \<in> \<R> l" "[r\<rightarrow>0]v \<in> zone_set R r"
-      unfolding zone_set_def region_set'_def by auto
-      from * have "Z \<inter> R \<noteq> {}" unfolding cla_def by auto
-      then have "zone_set (Z \<inter> R) r \<noteq> {}" unfolding zone_set_def by auto
-      from closure_id'[OF this _ ***(1)] have "Closure\<^sub>\<alpha>\<^sub>,\<^sub>l(zone_set (Z \<inter> R) r) = zone_set R r"
-      unfolding zone_set_def by auto
-      with v' **(1) have False by auto
-    }
-    then have "zone_set (Closure\<^sub>\<alpha>\<^sub>,\<^sub>l (Z \<inter> R)) r \<subseteq> Closure\<^sub>\<alpha>\<^sub>,\<^sub>l(zone_set (Z \<inter> R) r)" by auto
-  } note Z_i = this
-  from U(1) have "Closure\<^sub>\<alpha>\<^sub>,\<^sub>l Z = \<Union> {Closure\<^sub>\<alpha>\<^sub>,\<^sub>l (Z \<inter> R) | R. R \<in> U}" unfolding cla_def by auto
-  then have "zone_set (Closure\<^sub>\<alpha>\<^sub>,\<^sub>l Z) r = \<Union> {zone_set (Closure\<^sub>\<alpha>\<^sub>,\<^sub>l (Z \<inter> R)) r | R. R \<in> U}"
-  unfolding zone_set_def by auto
-  also have "\<dots> \<subseteq> \<Union> {Closure\<^sub>\<alpha>\<^sub>,\<^sub>l(zone_set (Z \<inter> R) r) | R. R \<in> U}" using Z_i by auto
-  also have "\<dots> = Closure\<^sub>\<alpha>\<^sub>,\<^sub>l \<Union> {(zone_set (Z \<inter> R) r) | R. R \<in> U}" unfolding cla_def by auto
-  also have "\<dots> = Closure\<^sub>\<alpha>\<^sub>,\<^sub>l (zone_set (\<Union> {Z \<inter> R| R. R \<in> U}) r)"
-  proof goal_cases
-    case 1
-    have "zone_set (\<Union> {Z \<inter> R| R. R \<in> U}) r = \<Union> {(zone_set (Z \<inter> R) r) | R. R \<in> U}"
-    unfolding zone_set_def by auto
-    then show ?case by auto
-  qed
-  finally show "zone_set (Closure\<^sub>\<alpha>\<^sub>,\<^sub>l Z) r \<subseteq> Closure\<^sub>\<alpha>\<^sub>,\<^sub>l(zone_set Z r)" using U by simp
-qed
-
-lemma SuccI3:
-  "R \<in> (\<R> l) \<Longrightarrow> v \<in> R \<Longrightarrow> t \<ge> 0 \<Longrightarrow> (v \<oplus> t) \<in> R' \<Longrightarrow> R' \<in> (\<R> l) \<Longrightarrow> R' \<in> Succ (\<R> l) R"
- apply (intro SuccI2[of "\<R> l" X "k l", folded \<R>_def, simplified])
-    apply assumption+
-   apply (intro region_unique[of "\<R> l" X "k l", folded \<R>_def, simplified, symmetric])
-by assumption+
-
-lemma closure_delay_mono:
-  "Z \<subseteq> V \<Longrightarrow> (Closure\<^sub>\<alpha>\<^sub>,\<^sub>l Z)\<^sup>\<up> \<subseteq> Closure\<^sub>\<alpha>\<^sub>,\<^sub>l (Z\<^sup>\<up>)"
-proof
-  fix v assume v: "v \<in> (Closure\<^sub>\<alpha>\<^sub>,\<^sub>l Z)\<^sup>\<up>" and Z: "Z \<subseteq> V"
-  then obtain u u' t R where A:
-    "u \<in> Closure\<^sub>\<alpha>\<^sub>,\<^sub>l Z" "v = (u \<oplus> t)" "u \<in> R" "u' \<in> R" "R \<in> \<R> l" "u' \<in> Z" "t \<ge> 0"
-  unfolding cla_def zone_delay_def by blast
-  from A(3,5) have "\<forall> x \<in> X. u x \<ge> 0" unfolding \<R>_def by fastforce
-  with region_cover_spec[of v] A(2,7) obtain R' where R':
-    "R' \<in> \<R> l" "v \<in> R'"
-  unfolding cval_add_def by auto
-  with set_of_regions_spec[OF A(5,4), OF SuccI3, of u] A obtain t where t:
-    "t \<ge> 0" "[u' \<oplus> t]\<^sub>\<R> l = R'"
-  by auto
-  with A have "(u' \<oplus> t) \<in> Z\<^sup>\<up>" unfolding zone_delay_def by auto
-  moreover from regions_closed'_spec[OF A(5,4)] t have "(u' \<oplus> t) \<in> R'" by auto
-  ultimately have "R' \<inter> (Z\<^sup>\<up>) \<noteq> {}" by auto
-  with R' show "v \<in> Closure\<^sub>\<alpha>\<^sub>,\<^sub>l (Z\<^sup>\<up>)" unfolding cla_def by auto
-qed
-
-lemma region_V: "R \<in> \<R> l \<Longrightarrow> R \<subseteq> V" using V_def \<R>_def region.cases by auto
-
-lemma closure_V:
-  "Closure\<^sub>\<alpha>\<^sub>,\<^sub>l Z \<subseteq> V"
-unfolding cla_def using region_V by auto
-
-lemma closure_V_int:
-  "Closure\<^sub>\<alpha>\<^sub>,\<^sub>l Z = Closure\<^sub>\<alpha>\<^sub>,\<^sub>l (Z \<inter> V)"
-unfolding cla_def using region_V by auto
-
-lemma closure_constraint_mono:
-  "Closure\<^sub>\<alpha>\<^sub>,\<^sub>l g = g \<Longrightarrow> g \<inter> (Closure\<^sub>\<alpha>\<^sub>,\<^sub>l Z) \<subseteq> Closure\<^sub>\<alpha>\<^sub>,\<^sub>l (g \<inter> Z)"
-unfolding cla_def by auto
-
-lemma closure_constraint_mono':
-  assumes "Closure\<^sub>\<alpha>\<^sub>,\<^sub>l g = g \<inter> V"
-  shows "g \<inter> (Closure\<^sub>\<alpha>\<^sub>,\<^sub>l Z) \<subseteq> Closure\<^sub>\<alpha>\<^sub>,\<^sub>l (g \<inter> Z)"
-proof -
-  from assms closure_V_int have "Closure\<^sub>\<alpha>\<^sub>,\<^sub>l (g \<inter> V) = g \<inter> V" by auto
-  from closure_constraint_mono[OF this, of Z] have
-    "g \<inter> (V \<inter> Closure\<^sub>\<alpha>\<^sub>,\<^sub>l Z) \<subseteq> Closure\<^sub>\<alpha>\<^sub>,\<^sub>l (g \<inter> Z \<inter> V)"
-  by (metis Int_assoc Int_commute)
-  with closure_V[of Z] closure_V_int[of "g \<inter> Z"] show ?thesis by auto
-qed
-
-lemma cla_empty_iff:
-  "Z \<subseteq> V \<Longrightarrow> Z = {} \<longleftrightarrow> Closure\<^sub>\<alpha>\<^sub>,\<^sub>l Z = {}"
-unfolding cla_def V_def using region_cover_spec by fast
-
-lemma closure_involutive_aux:
-  "U \<subseteq> \<R> l \<Longrightarrow> Closure\<^sub>\<alpha>\<^sub>,\<^sub>l \<Union> U = \<Union> U"
-unfolding cla_def using valid_regions_distinct_spec by blast
-
-lemma closure_involutive_aux':
-  "\<exists> U. U \<subseteq> \<R> l \<and> Closure\<^sub>\<alpha>\<^sub>,\<^sub>l Z = \<Union> U"
-unfolding cla_def by (rule exI[where x = "{R \<in> \<R> l. R \<inter> Z \<noteq> {}}"]) auto
-
-lemma closure_involutive:
-  "Closure\<^sub>\<alpha>\<^sub>,\<^sub>l Closure\<^sub>\<alpha>\<^sub>,\<^sub>l Z = Closure\<^sub>\<alpha>\<^sub>,\<^sub>l Z"
-using closure_involutive_aux closure_involutive_aux' by metis
-
-lemma closure_involutive':
-  "Z \<subseteq> Closure\<^sub>\<alpha>\<^sub>,\<^sub>l W \<Longrightarrow> Closure\<^sub>\<alpha>\<^sub>,\<^sub>l Z \<subseteq> Closure\<^sub>\<alpha>\<^sub>,\<^sub>l W"
-unfolding cla_def using valid_regions_distinct_spec by fast
-
-lemma closure_subs:
-  "Z \<subseteq> V \<Longrightarrow> Z \<subseteq> Closure\<^sub>\<alpha>\<^sub>,\<^sub>l Z"
-unfolding cla_def V_def using region_cover_spec by fast
-
-lemma cla_mono':
-  "Z' \<subseteq> V \<Longrightarrow> Z \<subseteq> Z' \<Longrightarrow> Closure\<^sub>\<alpha>\<^sub>,\<^sub>l Z \<subseteq> Closure\<^sub>\<alpha>\<^sub>,\<^sub>l Z'"
-by (meson closure_involutive' closure_subs subset_trans)
-
-lemma cla_mono:
-  "Z \<subseteq> Z' \<Longrightarrow> Closure\<^sub>\<alpha>\<^sub>,\<^sub>l Z \<subseteq> Closure\<^sub>\<alpha>\<^sub>,\<^sub>l Z'"
-using closure_V_int cla_mono'[of "Z' \<inter> V" "Z \<inter> V"] by auto
-
-end
 
 section \<open>A New Zone Semantics Abstracting with \<open>Closure\<^sub>\<alpha>\<^sub>,\<^sub>l\<close>\<close>
 
@@ -955,22 +773,6 @@ inductive_cases[elim!]: "A \<turnstile> \<langle>l, u\<rangle> \<leadsto>\<^bsub
 
 declare step_z_alpha.intros[intro]
 
-lemma up_V: "Z \<subseteq> V \<Longrightarrow> Z\<^sup>\<up> \<subseteq> V"
-unfolding V_def zone_delay_def cval_add_def by auto
-
-lemma reset_V: "Z \<subseteq> V \<Longrightarrow> (zone_set Z r) \<subseteq> V"
-unfolding V_def unfolding zone_set_def by (induction r, auto)
-
-lemma step_z_V: "A \<turnstile> \<langle>l, Z\<rangle> \<leadsto>\<^bsub>a\<^esub> \<langle>l',Z'\<rangle> \<Longrightarrow> Z \<subseteq> V \<Longrightarrow> Z' \<subseteq> V"
- apply (induction rule: step_z.induct)
-  apply (rule le_infI1)
-  apply (rule up_V)
-  apply blast
- apply (rule le_infI1)
- apply (rule reset_V)
-by blast
-
-
 text \<open>Single-step soundness and completeness follows trivially from \<open>cla_empty_iff\<close>.\<close>
 
 lemma step_z_alpha_sound:
@@ -980,8 +782,17 @@ lemma step_z_alpha_sound:
   apply (frule step_z_V)
   apply assumption
  apply (rotate_tac 3)
- apply (drule cla_empty_iff)
-by auto
+ by (fastforce simp: cla_def)
+
+context
+  fixes l l' :: 's
+begin
+
+interpretation alpha: AlphaClosure_global _ "k l'" "\<R> l'" by standard (rule finite)
+
+lemma [simp]:
+  "alpha.cla = cla l'"
+  unfolding cla_def alpha.cla_def ..
 
 lemma step_z_alpha_complete:
   "A \<turnstile> \<langle>l, Z\<rangle> \<leadsto>\<^bsub>a\<^esub> \<langle>l',Z'\<rangle> \<Longrightarrow> Z \<subseteq> V \<Longrightarrow> Z' \<noteq> {}
@@ -989,8 +800,10 @@ lemma step_z_alpha_complete:
   apply (frule step_z_V)
    apply assumption
   apply (rotate_tac 3)
-  apply (drule cla_empty_iff[where l = l'])
+  apply (drule alpha.cla_empty_iff)
   by auto
+
+end (* End of context for global closure proofs *)
 
 subsection \<open>Multi step\<close>
 
@@ -1007,163 +820,30 @@ declare steps_z_alpha.intros[intro]
 text \<open>P. Bouyer's calculation for @{term "Post(Closure\<^sub>\<alpha>\<^sub>,\<^sub>l Z, e) \<subseteq> Closure\<^sub>\<alpha>\<^sub>,\<^sub>l(Post (Z, e))"}\<close>
 text \<open>This is now obsolete as we argue solely with monotonicty of \<open>steps_z\<close> w.r.t \<open>Closure\<^sub>\<alpha>\<^sub>,\<^sub>l\<close>\<close>
 
-(*
-lemma calc:
-  "valid_abstraction A X k \<Longrightarrow> Z \<subseteq> V \<Longrightarrow> A \<turnstile> \<langle>l, Closure\<^sub>\<alpha>\<^sub>,\<^sub>l Z\<rangle> \<leadsto>\<^bsub>a\<^esub> \<langle>l', Z'\<rangle>
-  \<Longrightarrow> \<exists>Z''. A \<turnstile> \<langle>l, Z\<rangle> \<leadsto>\<^bsub>\<alpha>(a)\<^esub> \<langle>l', Z''\<rangle> \<and> Z' \<subseteq> Z''"
-proof (cases rule: step_z.cases, assumption, goal_cases)
-  case 1
-  note A = this
-  from A(1) have "\<forall>(x, m)\<in>clkp_set A l. m \<le> real (k l x) \<and> x \<in> X \<and> m \<in> \<nat>"
-  by (fastforce elim: valid_abstraction.cases)
-  then have "\<forall>(x, m)\<in>collect_clock_pairs (inv_of A l). m \<le> real (k x) \<and> x \<in> X \<and> m \<in> \<nat>"
-  unfolding clkp_set_def collect_clki_def inv_of_def by auto
-  from closure_constraint_id[OF this] have *: "Closure\<^sub>\<alpha>\<^sub>,\<^sub>l \<lbrace>inv_of A l\<rbrace> = \<lbrace>inv_of A l\<rbrace> \<inter> V" .
-  have "(Closure\<^sub>\<alpha>\<^sub>,\<^sub>l Z)\<^sup>\<up> \<subseteq> Closure\<^sub>\<alpha>\<^sub>,\<^sub>l (Z\<^sup>\<up>)" using A(2) by (blast intro!: closure_delay_mono)
-  then have "Z' \<subseteq> Closure\<^sub>\<alpha>\<^sub>,\<^sub>l (Z\<^sup>\<up> \<inter> {u. u \<turnstile> inv_of A l})"
-  using closure_constraint_mono'[OF *, of "Z\<^sup>\<up>"] unfolding ccval_def by (auto simp: Int_commute A(6))
-  with A(4,3) show ?thesis by auto
-next
-  case (2 g a r)
-  note A = this
-  from A(1) have *:
-    "\<forall>(x, m)\<in>clkp_set A. m \<le> real (k x) \<and> x \<in> X \<and> m \<in> \<nat>"
-    "collect_clkvt (trans_of A) \<subseteq> X"
-    "finite X"
-  by (auto elim: valid_abstraction.cases)
-  from *(1) A(5) have "\<forall>(x, m)\<in>collect_clock_pairs (inv_of A l'). m \<le> real (k x) \<and> x \<in> X \<and> m \<in> \<nat>"
-  unfolding clkp_set_def collect_clki_def inv_of_def by fastforce
-  from closure_constraint_id[OF this] have **: "Closure\<^sub>\<alpha>\<^sub>,\<^sub>l \<lbrace>inv_of A l'\<rbrace> = \<lbrace>inv_of A l'\<rbrace> \<inter> V" .
-  from *(1) A(6) have "\<forall>(x, m)\<in>collect_clock_pairs g. m \<le> real (k x) \<and> x \<in> X \<and> m \<in> \<nat>"
-  unfolding clkp_set_def collect_clkt_def by fastforce
-  from closure_constraint_id[OF this] have ***: "Closure\<^sub>\<alpha>\<^sub>,\<^sub>l \<lbrace>g\<rbrace> = \<lbrace>g\<rbrace> \<inter> V" .
-  from *(2) A(6) have ****: "set r \<subseteq> X" unfolding collect_clkvt_def by fastforce
-  from closure_constraint_mono'[OF ***, of Z] have
-    "(Closure\<^sub>\<alpha>\<^sub>,\<^sub>l Z) \<inter> {u. u \<turnstile> g} \<subseteq> Closure\<^sub>\<alpha>\<^sub>,\<^sub>l (Z \<inter> {u. u \<turnstile> g})" unfolding ccval_def
-  by (subst Int_commute) (subst (asm) (2) Int_commute, assumption)
-  moreover have "zone_set \<dots> r \<subseteq> Closure\<^sub>\<alpha>\<^sub>,\<^sub>l (zone_set (Z \<inter> {u. u \<turnstile> g}) r)" using **** A(2)
-  by (intro closure_update_mono, auto)
-  ultimately have "Z' \<subseteq> Closure\<^sub>\<alpha>\<^sub>,\<^sub>l (zone_set (Z \<inter> {u. u \<turnstile> g}) r \<inter> {u. u \<turnstile> inv_of A l'})"
-  using closure_constraint_mono'[OF **, of "zone_set (Z \<inter> {u. u \<turnstile> g}) r"] unfolding ccval_def
-    apply (subst A(5))
-    apply (subst (asm) (5 7) Int_commute)
-    apply (rule subset_trans)
-     defer
-     apply assumption
-    apply (subst subset_int_mono)
-     defer
-     apply rule
-    apply (rule subset_trans)
-     defer
-     apply assumption
-    apply (rule zone_set_mono)
-    apply assumption
-  done
-  with A(6) show ?thesis by (auto simp: A(4))
-qed
-*)
-
 text \<open>
   Turning P. Bouyers argument for multiple steps into an inductive proof is not direct.
   With this initial argument we can get to a point where the induction hypothesis is applicable.
   This breaks the "information hiding" induced by the different variants of steps.
 \<close>
-(*
-lemma steps_z_alpha_closure_involutive'_aux:
-  "A \<turnstile> \<langle>l, Z\<rangle> \<leadsto>\<^bsub>a\<^esub> \<langle>l',Z'\<rangle> \<Longrightarrow> Closure\<^sub>\<alpha>\<^sub>,\<^sub>l Z \<subseteq> Closure\<^sub>\<alpha>\<^sub>,\<^sub>l W \<Longrightarrow> valid_abstraction A X k \<Longrightarrow> Z \<subseteq> V
-  \<Longrightarrow> \<exists> W'. A \<turnstile> \<langle>l, W\<rangle> \<leadsto>\<^bsub>a\<^esub> \<langle>l',W'\<rangle> \<and> Closure\<^sub>\<alpha>\<^sub>,\<^sub>l Z' \<subseteq> Closure\<^sub>\<alpha>\<^sub>,\<^sub>l W'"
-proof (induction rule: step_z.induct)
-  case A: (step_t_z A l Z)
-  let ?Z' = "Z\<^sup>\<up> \<inter> {u. u \<turnstile> inv_of A l}"
-  let ?W' = "W\<^sup>\<up> \<inter> {u. u \<turnstile> inv_of A l}"
-  from \<R>_def have \<R>_def': "\<R> = {region X I r |I r. valid_region X k I r}" by simp
-  have step_z: "A \<turnstile> \<langle>l, W\<rangle> \<leadsto>\<^bsub>\<tau>\<^esub> \<langle>l,?W'\<rangle>" by auto
-  moreover have "Closure\<^sub>\<alpha>\<^sub>,\<^sub>l ?Z' \<subseteq> Closure\<^sub>\<alpha>\<^sub>,\<^sub>l ?W'"
-  proof
-    fix v assume v: "v \<in> Closure\<^sub>\<alpha>\<^sub>,\<^sub>l ?Z'"
-    then obtain R' v' where 1: "R' \<in> \<R>" "v \<in> R'" "v' \<in> R'" "v' \<in> ?Z'" unfolding cla_def by auto
-    then obtain u d where
-      "u \<in> Z" and v': "v' = u \<oplus> d" "u \<oplus> d \<turnstile> inv_of A l" "0 \<le> d"
-    unfolding zone_delay_def by blast
-    with closure_subs[OF A(3)] A(1) obtain u' R where u': "u' \<in> W" "u \<in> R" "u' \<in> R" "R \<in> \<R>"
-    unfolding cla_def by blast
-    then have "\<forall>x\<in>X. 0 \<le> u x" unfolding \<R>_def by fastforce
-    from region_cover'[OF \<R>_def' this] have R: "[u]\<^sub>\<R> \<in> \<R>" "u \<in> [u]\<^sub>\<R>" by auto
-    from SuccI2[OF \<R>_def' this(2,1) \<open>0 \<le> d\<close>, of "[v']\<^sub>\<R>"] v'(1) have v'1:
-      "[v']\<^sub>\<R> \<in> Succ \<R> ([u]\<^sub>\<R>)" "[v']\<^sub>\<R> \<in> \<R>"
-    by auto
-    from regions_closed'_spec[OF R(1,2) \<open>0 \<le> d\<close>] v'(1) have v'2: "v' \<in> [v']\<^sub>\<R>" by simp
-    from A(2) have *:
-      "\<forall>(x, m)\<in>clkp_set A. m \<le> real (k x) \<and> x \<in> X \<and> m \<in> \<nat>"
-      "collect_clkvt (trans_of A) \<subseteq> X"
-      "finite X"
-    by (auto elim: valid_abstraction.cases)
-    from *(1) u'(2) have "\<forall>(x, m)\<in>collect_clock_pairs (inv_of A l). m \<le> real (k x) \<and> x \<in> X \<and> m \<in> \<nat>"
-    unfolding clkp_set_def collect_clki_def inv_of_def by fastforce
-    from ccompatible[OF this, folded \<R>_def'] v'1(2) v'2 v'(1,2) have 3:
-      "[v']\<^sub>\<R> \<subseteq> \<lbrace>inv_of A l\<rbrace>"
-    unfolding ccompatible_def ccval_def by auto
-    with A v'1 R(1) \<R>_def' have "A,\<R> \<turnstile> \<langle>l, ([u]\<^sub>\<R>)\<rangle> \<leadsto> \<langle>l,([v']\<^sub>\<R>)\<rangle>" by auto
-    with valid_regions_distinct_spec[OF v'1(2) 1(1) v'2 1(3)] region_unique_spec[OF u'(2,4)]
-    have step_r: "A,\<R> \<turnstile> \<langle>l, R\<rangle> \<leadsto> \<langle>l, R'\<rangle>" and 2: "[v']\<^sub>\<R> = R'" "[u]\<^sub>\<R> = R" by auto
-    from set_of_regions_spec[OF u'(4,3)] v'1(1) 2 obtain t where t: "t \<ge> 0" "[u' \<oplus> t]\<^sub>\<R> = R'" by auto
-    with regions_closed'_spec[OF u'(4,3) this(1)] step_t_r(1) have *: "u' \<oplus> t \<in> R'" by auto
-    with t(1) 3 2 u'(1,3) have "A \<turnstile> \<langle>l, u'\<rangle> \<rightarrow> \<langle>l, u' \<oplus> t\<rangle>" "u' \<oplus> t \<in> ?W'"
-    unfolding zone_delay_def ccval_def by auto
-    with * 1(1) have "R' \<subseteq> Closure\<^sub>\<alpha>\<^sub>,\<^sub>l ?W'" unfolding cla_def by auto
-    with 1(2) show "v \<in> Closure\<^sub>\<alpha>\<^sub>,\<^sub>l ?W'" ..
-  qed
-  ultimately show ?case by auto
-next
-  case A: (step_a_z A l g a r l' Z)
-  let ?Z' = "zone_set (Z \<inter> {u. u \<turnstile> g}) r \<inter> {u. u \<turnstile> inv_of A l'}"
-  let ?W' = "zone_set (W \<inter> {u. u \<turnstile> g}) r \<inter> {u. u \<turnstile> inv_of A l'}"
-  from \<R>_def have \<R>_def': "\<R> = {region X I r |I r. valid_region X k I r}" by simp
-  from A(1) have step_z: "A \<turnstile> \<langle>l, W\<rangle> \<leadsto>\<^bsub>\<upharpoonleft>a\<^esub> \<langle>l',?W'\<rangle>" by auto
-  moreover have "Closure\<^sub>\<alpha>\<^sub>,\<^sub>l ?Z' \<subseteq> Closure\<^sub>\<alpha>\<^sub>,\<^sub>l ?W'"
-  proof
-    fix v assume v: "v \<in> Closure\<^sub>\<alpha>\<^sub>,\<^sub>l ?Z'"
-    then obtain R' v' where 1: "R' \<in> \<R>" "v \<in> R'" "v' \<in> R'" "v' \<in> ?Z'" unfolding cla_def by auto
-    then obtain u where
-      "u \<in> Z" and v': "v' = [r\<rightarrow>0]u" "u \<turnstile> g" "v' \<turnstile> inv_of A l'"
-    unfolding zone_set_def by blast
-    let ?R'= "region_set' (([u]\<^sub>\<R>) \<inter> {u. u \<turnstile> g}) r 0 \<inter> {u. u \<turnstile> inv_of A l'}"
-    from \<open>u \<in> Z\<close> closure_subs[OF A(4)] A(2) obtain u' R where u': "u' \<in> W" "u \<in> R" "u' \<in> R" "R \<in> \<R>"
-    unfolding cla_def by blast
-    then have "\<forall>x\<in>X. 0 \<le> u x" unfolding \<R>_def by fastforce
-    from region_cover'[OF \<R>_def' this] have R: "[u]\<^sub>\<R> \<in> \<R>" "u \<in> [u]\<^sub>\<R>" by auto
-    from step_r_complete_aux[OF \<R>_def' A(3) this(2,1) A(1) v'(2)] v'
-    have *: "[u]\<^sub>\<R> = ([u]\<^sub>\<R>) \<inter> {u. u \<turnstile> g}" "?R' = region_set' ([u]\<^sub>\<R>) r 0" "?R' \<in> \<R>" by auto
-    from \<R>_def' A(3) have "collect_clkvt (trans_of A) \<subseteq> X" "finite X"
-    by (auto elim: valid_abstraction.cases)
-    with A(1) have r: "set r \<subseteq> X" unfolding collect_clkvt_def by fastforce
-    from * v'(1) R(2) have "v' \<in> ?R'" unfolding region_set'_def by auto
-    moreover have "A,\<R> \<turnstile> \<langle>l,([u]\<^sub>\<R>)\<rangle> \<leadsto> \<langle>l',?R'\<rangle>" using R(1) \<R>_def' A(1,3) v'(2) by auto
-    thm valid_regions_distinct_spec
-    with valid_regions_distinct_spec[OF *(3) 1(1) \<open>v' \<in> ?R'\<close> 1(3)] region_unique_spec[OF u'(2,4)]
-    have 2: "?R' = R'" "[u]\<^sub>\<R> = R" by auto
-    with * u' have *: "[r\<rightarrow>0]u' \<in> ?R'" "u' \<turnstile> g" "[r\<rightarrow>0]u' \<turnstile> inv_of A l'"
-    unfolding region_set'_def by auto
-    with A(1) have "A \<turnstile> \<langle>l, u'\<rangle> \<rightarrow> \<langle>l',[r\<rightarrow>0]u'\<rangle>" apply (intro step.intros(1)) apply rule by auto
-    moreover from * u'(1) have "[r\<rightarrow>0]u' \<in> ?W'" unfolding zone_set_def by auto
-    ultimately have "R' \<subseteq> Closure\<^sub>\<alpha>\<^sub>,\<^sub>l ?W'" using *(1) 1(1) 2(1) unfolding cla_def by auto
-    with 1(2) show "v \<in> Closure\<^sub>\<alpha>\<^sub>,\<^sub>l ?W'" ..
-  qed
-  ultimately show ?case by meson
-qed
-*)
 
 context
+  fixes l l' :: 's
 begin
 
-abbreviation part'' ("[_]\<^sub>_" [61,61] 61) where "part'' u l \<equiv> part u (\<R> l)"
+interpretation alpha: AlphaClosure_global _ "k l" "\<R> l" by standard (rule finite)
+lemma [simp]: "alpha.cla = cla l" unfolding alpha.cla_def cla_def ..
+
+interpretation alpha': AlphaClosure_global _ "k l'" "\<R> l'" by standard (rule finite)
+lemma [simp]: "alpha'.cla = cla l'" unfolding alpha'.cla_def cla_def ..
+
+abbreviation part'' ("[_]\<^sub>_" [61,61] 61) where "part'' u l1 \<equiv> part u (\<R> l1)"
 no_notation part ("[_]\<^sub>_" [61,61] 61)
 
 lemma steps_z_alpha_closure_involutive'_aux':
   "A \<turnstile> \<langle>l, Z\<rangle> \<leadsto>\<^bsub>a\<^esub> \<langle>l',Z'\<rangle> \<Longrightarrow> Closure\<^sub>\<alpha>\<^sub>,\<^sub>l Z \<subseteq> Closure\<^sub>\<alpha>\<^sub>,\<^sub>l W \<Longrightarrow> valid_abstraction A X k \<Longrightarrow> Z \<subseteq> V \<Longrightarrow> W \<subseteq> Z
   \<Longrightarrow> \<exists> W'. A \<turnstile> \<langle>l, W\<rangle> \<leadsto>\<^bsub>a\<^esub> \<langle>l',W'\<rangle> \<and> Closure\<^sub>\<alpha>\<^sub>,\<^sub>l' Z' \<subseteq> Closure\<^sub>\<alpha>\<^sub>,\<^sub>l' W' \<and> W' \<subseteq> Z'"
-proof (induction rule: step_z.induct)
-  case A: (step_t_z A l Z)
+proof (induction A \<equiv> A l \<equiv> l _ _ l' \<equiv> l' _rule: step_z.induct)
+  case A: (step_t_z Z)
   let ?Z' = "Z\<^sup>\<up> \<inter> {u. u \<turnstile> inv_of A l}"
   let ?W' = "W\<^sup>\<up> \<inter> {u. u \<turnstile> inv_of A l}"
   from \<R>_def have \<R>_def': "\<R> l = {region X I r |I r. valid_region X (k l) I r}" for l by simp
@@ -1175,15 +855,16 @@ proof (induction rule: step_z.induct)
     then obtain u d where
       "u \<in> Z" and v': "v' = u \<oplus> d" "u \<oplus> d \<turnstile> inv_of A l" "0 \<le> d"
     unfolding zone_delay_def by blast
-    with closure_subs[OF A(3)] A(1) obtain u' R where u': "u' \<in> W" "u \<in> R" "u' \<in> R" "R \<in> \<R> l"
-    unfolding cla_def by blast
+    with alpha.closure_subs[OF A(4)] A(2) obtain u' R where u':
+      "u' \<in> W" "u \<in> R" "u' \<in> R" "R \<in> \<R> l"
+    by (simp add: cla_def) blast
     then have "\<forall>x\<in>X. 0 \<le> u x" unfolding \<R>_def by fastforce
     from region_cover'[OF \<R>_def' this] have R: "[u]\<^sub>l \<in> \<R> l" "u \<in> [u]\<^sub>l" by auto
     from SuccI2[OF \<R>_def' this(2,1) \<open>0 \<le> d\<close>, of "[v']\<^sub>l"] v'(1) have v'1:
       "[v']\<^sub>l \<in> Succ (\<R> l) ([u]\<^sub>l)" "[v']\<^sub>l \<in> \<R> l"
     by auto
-    from regions_closed'_spec[OF R(1,2) \<open>0 \<le> d\<close>] v'(1) have v'2: "v' \<in> [v']\<^sub>l" by simp
-    from A(2) have
+    from alpha.regions_closed'_spec[OF R(1,2) \<open>0 \<le> d\<close>] v'(1) have v'2: "v' \<in> [v']\<^sub>l" by simp
+    from A(3) have
       "\<forall>(x, m)\<in>clkp_set A l. m \<le> real (k l x) \<and> x \<in> X \<and> m \<in> \<nat>"
     by (auto elim!: valid_abstraction.cases)
     then have
@@ -1192,20 +873,22 @@ proof (induction rule: step_z.induct)
     from ccompatible[OF this, folded \<R>_def'] v'1(2) v'2 v'(1,2) have 3:
       "[v']\<^sub>l \<subseteq> \<lbrace>inv_of A l\<rbrace>"
     unfolding ccompatible_def ccval_def by auto
-    from valid_regions_distinct_spec[OF v'1(2) 1(1) v'2 1(3)] region_unique_spec[OF u'(2,4)]
+    from
+      alpha.valid_regions_distinct_spec[OF v'1(2) 1(1) v'2 1(3)]
+      alpha.region_unique_spec[OF u'(2,4)]
     have 2: "[v']\<^sub>l = R'" "[u]\<^sub>l = R" by auto
-    from set_of_regions_spec[OF u'(4,3)] v'1(1) 2 obtain t where t:
+    from alpha.set_of_regions_spec[OF u'(4,3)] v'1(1) 2 obtain t where t:
       "t \<ge> 0" "[u' \<oplus> t]\<^sub>l = R'" by auto
-    with regions_closed'_spec[OF u'(4,3) this(1)] step_t_r(1) have *: "u' \<oplus> t \<in> R'" by auto
+    with alpha.regions_closed'_spec[OF u'(4,3) this(1)] step_t_r(1) have *: "u' \<oplus> t \<in> R'" by auto
     with t(1) 3 2 u'(1,3) have "A \<turnstile> \<langle>l, u'\<rangle> \<rightarrow> \<langle>l, u' \<oplus> t\<rangle>" "u' \<oplus> t \<in> ?W'"
     unfolding zone_delay_def ccval_def by auto
     with * 1(1) have "R' \<subseteq> Closure\<^sub>\<alpha>\<^sub>,\<^sub>l ?W'" unfolding cla_def by auto
     with 1(2) show "v \<in> Closure\<^sub>\<alpha>\<^sub>,\<^sub>l ?W'" ..
   qed
   moreover have "?W' \<subseteq> ?Z'" using \<open>W \<subseteq> Z\<close> unfolding zone_delay_def by auto
-  ultimately show ?case by auto
+  ultimately show ?case unfolding \<open>l = l'\<close> by auto
 next
-  case A: (step_a_z A l g a r l' Z)
+  case A: (step_a_z g a r Z)
   let ?Z' = "zone_set (Z \<inter> {u. u \<turnstile> g}) r \<inter> {u. u \<turnstile> inv_of A l'}"
   let ?W' = "zone_set (W \<inter> {u. u \<turnstile> g}) r \<inter> {u. u \<turnstile> inv_of A l'}"
   from \<R>_def have \<R>_def': "\<R> l = {region X I r |I r. valid_region X (k l) I r}" for l by simp
@@ -1218,9 +901,9 @@ next
       "u \<in> Z" and v': "v' = [r\<rightarrow>0]u" "u \<turnstile> g" "v' \<turnstile> inv_of A l'"
     unfolding zone_set_def by blast
     let ?R'= "region_set' (([u]\<^sub>l) \<inter> {u. u \<turnstile> g}) r 0 \<inter> {u. u \<turnstile> inv_of A l'}"
-    from \<open>u \<in> Z\<close> closure_subs[OF A(4)] A(2) obtain u' R where u':
+    from \<open>u \<in> Z\<close> alpha.closure_subs[OF A(4)] A(2) obtain u' R where u':
       "u' \<in> W" "u \<in> R" "u' \<in> R" "R \<in> \<R> l"
-    unfolding cla_def by blast
+    by (simp add: cla_def) blast
     then have "\<forall>x\<in>X. 0 \<le> u x" unfolding \<R>_def by fastforce
     from region_cover'[OF \<R>_def' this] have "[u]\<^sub>l \<in> \<R> l" "u \<in> [u]\<^sub>l" by auto
     have *:
@@ -1247,7 +930,7 @@ next
         "[u]\<^sub>l = ([u]\<^sub>l) \<inter> {u. u \<turnstile> g}"
         unfolding ccompatible_def ccval_def by blast
       have **: "[r\<rightarrow>0]u \<in> [[r\<rightarrow>0]u]\<^sub>l'"
-        using \<open>R' \<in> \<R> l'\<close> \<open>v' \<in> R'\<close> region_unique_spec v'(1) by blast
+        using \<open>R' \<in> \<R> l'\<close> \<open>v' \<in> R'\<close> alpha'.region_unique_spec v'(1) by blast
       from * have
         "\<forall>(x, m)\<in>collect_clock_pairs (inv_of A l'). m \<le> real (k l' x) \<and> x \<in> X \<and> m \<in> \<nat>"
         unfolding inv_of_def clkp_set_def collect_clki_def by fastforce
@@ -1256,9 +939,9 @@ next
         unfolding ccompatible_def ccval_def \<open>v' = _\<close> by blast
     qed
     from * \<open>v' = _\<close> \<open>u \<in> [u]\<^sub>l\<close> have "v' \<in> [[r\<rightarrow>0]u]\<^sub>l'" unfolding region_set'_def by auto
-    from valid_regions_distinct_spec[OF *(3) \<open>R' \<in> \<R> l'\<close> \<open>v' \<in> [[r\<rightarrow>0]u]\<^sub>l'\<close> \<open>v' \<in> R'\<close>]
+    from alpha'.valid_regions_distinct_spec[OF *(3) \<open>R' \<in> \<R> l'\<close> \<open>v' \<in> [[r\<rightarrow>0]u]\<^sub>l'\<close> \<open>v' \<in> R'\<close>]
     have "[[r\<rightarrow>0]u]\<^sub>l' = R'" .
-    from region_unique_spec[OF u'(2,4)] have "[u]\<^sub>l = R" by auto
+    from alpha.region_unique_spec[OF u'(2,4)] have "[u]\<^sub>l = R" by auto
     from \<open>[u]\<^sub>l = R\<close> *(1,2) *(4) \<open>u' \<in> R\<close> have
       "[r\<rightarrow>0]u' \<in> [[r\<rightarrow>0]u]\<^sub>l'" "u' \<turnstile> g" "[r\<rightarrow>0]u' \<turnstile> inv_of A l'"
       unfolding region_set'_def by auto
@@ -1271,15 +954,20 @@ next
   ultimately show ?case by meson
 qed
 
-end (* End of context for special region notation *)
+lemma steps_z_alpha_V: "A \<turnstile> \<langle>l, Z\<rangle> \<leadsto>\<^sub>\<alpha>* \<langle>l',Z'\<rangle> \<Longrightarrow> Z \<subseteq> V \<Longrightarrow> Z' \<subseteq> V"
+  by(induction A \<equiv> A l \<equiv> l _ l' \<equiv> l' _ rule: steps_z_alpha.induct)
+    (auto intro!: alpha'.closure_V[simplified])
+
+lemma steps_z_V:
+  "A \<turnstile> \<langle>l, Z\<rangle> \<leadsto>* \<langle>l',Z'\<rangle> \<Longrightarrow> Z \<subseteq> V \<Longrightarrow> Z' \<subseteq> V"
+  using alpha'.steps_z_V .
+
+end (* End of context for special region notation and fixed locations *)
 
 lemma steps_z_alt:
   "A \<turnstile> \<langle>l, Z\<rangle> \<leadsto>* \<langle>l',Z'\<rangle> \<Longrightarrow> A \<turnstile> \<langle>l', Z'\<rangle> \<leadsto>\<^bsub>\<tau>\<^esub> \<langle>l'',Z''\<rangle> \<Longrightarrow> A \<turnstile> \<langle>l'', Z''\<rangle> \<leadsto>\<^bsub>\<upharpoonleft>a\<^esub> \<langle>l''',Z'''\<rangle>
   \<Longrightarrow> A \<turnstile> \<langle>l, Z\<rangle> \<leadsto>* \<langle>l''',Z'''\<rangle>"
 by (induction rule: steps_z.induct) auto
-
-lemma steps_z_alpha_V: "A \<turnstile> \<langle>l, Z\<rangle> \<leadsto>\<^sub>\<alpha>* \<langle>l',Z'\<rangle> \<Longrightarrow> Z \<subseteq> V \<Longrightarrow> Z' \<subseteq> V"
-by (induction rule: steps_z_alpha.induct) (auto intro!: closure_V)
 
 lemma steps_z_alpha_closure_involutive':
   "A \<turnstile> \<langle>l, Z\<rangle> \<leadsto>\<^sub>\<alpha>* \<langle>l', Z'\<rangle> \<Longrightarrow> A \<turnstile> \<langle>l', Z'\<rangle> \<leadsto>\<^bsub>\<tau>\<^esub> \<langle>l', Z''\<rangle> \<Longrightarrow> A \<turnstile> \<langle>l', Z''\<rangle> \<leadsto>\<^bsub>\<upharpoonleft>a\<^esub> \<langle>l'',Z'''\<rangle>
@@ -1289,19 +977,20 @@ proof (induction A l Z l' Z' arbitrary: a Z'' Z''' l'' rule: steps_z_alpha.induc
   case refl then show ?case by blast
 next
   case A: (2 A l Z l' Z' Z'' a l'' Z''' aa Z''a Z'''a l''')
+  interpret alpha'': AlphaClosure_global _ "k l''" "\<R> l''" by standard (rule finite)
+  have [simp]: \<open>alpha''.cla = cla l''\<close> unfolding alpha''.cla_def cla_def ..
+  note closure_V = alpha''.closure_V[simplified]
   from A(4) obtain \<Z> where Z''': "Z''' = Closure\<^sub>\<alpha>\<^sub>,\<^sub>l'' \<Z>" "A \<turnstile> \<langle>l', Z''\<rangle> \<leadsto>\<^bsub>\<upharpoonleft>a\<^esub> \<langle>l'', \<Z>\<rangle>" by auto
   from A(2)[OF A(3) this(2) A(7,8)] A(4) obtain W''' where W''':
     "A \<turnstile> \<langle>l, Z\<rangle> \<leadsto>* \<langle>l'',W'''\<rangle>" "Closure\<^sub>\<alpha>\<^sub>,\<^sub>l'' \<Z> \<subseteq> Closure\<^sub>\<alpha>\<^sub>,\<^sub>l'' W'''" "W''' \<subseteq> \<Z>"
     by auto
-  have "Z''a \<subseteq> V"
-    by (metis A(5) Z'''(1) closure_V step_z_V)
-  have "\<Z> \<subseteq> V"
-    by (meson A(1) A(3) A(8) Z'''(2) step_z_V steps_z_alpha_V)
-  from closure_subs[OF this] \<open>W''' \<subseteq> \<Z>\<close> have *: "W''' \<subseteq> Closure\<^sub>\<alpha>\<^sub>,\<^sub>l'' \<Z>" by auto
+  have "Z''a \<subseteq> V" by (metis A(5) Z'''(1) closure_V step_z_V)
+  have "\<Z> \<subseteq> V" by (meson A(1) A(3) A(8) Z'''(2) step_z_V steps_z_alpha_V)
+  from alpha''.closure_subs[OF this] \<open>W''' \<subseteq> \<Z>\<close> have *: "W''' \<subseteq> Closure\<^sub>\<alpha>\<^sub>,\<^sub>l'' \<Z>" by auto
   from A(5) \<open>Z''' = _\<close> have "A \<turnstile> \<langle>l'', Closure\<^sub>\<alpha>\<^sub>,\<^sub>l'' \<Z>\<rangle> \<leadsto>\<^bsub>\<tau>\<^esub> \<langle>l'', Z''a\<rangle>" by simp
   from steps_z_alpha_closure_involutive'_aux'[OF this _ A(7) closure_V *] W'''(2) obtain W'
     where ***: "A \<turnstile> \<langle>l'', W'''\<rangle> \<leadsto>\<^bsub>\<tau>\<^esub> \<langle>l'', W'\<rangle>" "Closure\<^sub>\<alpha>\<^sub>,\<^sub>l'' Z''a \<subseteq> Closure\<^sub>\<alpha>\<^sub>,\<^sub>l'' W'" "W' \<subseteq> Z''a"
-    by atomize_elim (auto simp: closure_involutive)
+    by atomize_elim (auto simp: alpha''.closure_involutive[simplified])
   text \<open>This shows how we could easily add more steps before doing the final closure operation!\<close>
   from steps_z_alpha_closure_involutive'_aux'[OF A(6) this(2) A(7) \<open>Z''a \<subseteq> V\<close> this(3)] obtain W''
     where
@@ -1310,32 +999,6 @@ next
   with *** W''' show ?case by (blast intro: steps_z_alt)
 qed
 
-(*
-text \<open>Old proof using Bouyer's calculation\<close>
-lemma steps_z_alpha_closure_involutive'':
-  "A \<turnstile> \<langle>l, Z\<rangle> \<leadsto>\<^sub>\<alpha>* \<langle>l',Z'\<rangle> \<Longrightarrow> A \<turnstile> \<langle>l', Z'\<rangle> \<leadsto> \<langle>l'',Z''\<rangle> \<Longrightarrow> valid_abstraction A X k \<Longrightarrow> Z \<subseteq> V
-  \<Longrightarrow> \<exists> Z'''. A \<turnstile> \<langle>l, Z\<rangle> \<leadsto>* \<langle>l'',Z'''\<rangle> \<and> Closure\<^sub>\<alpha>\<^sub>,\<^sub>l Z'' \<subseteq> Closure\<^sub>\<alpha>\<^sub>,\<^sub>l Z'''"
-proof (induction A l Z l' Z' arbitrary: Z'' l'' rule: steps_z_alpha.induct, goal_cases)
-  case refl from this(1) show ?case by blast
-next
-  case A: (2 A l Z l' Z' l'' Z'' Z''a l''a)
-  from A(3) obtain \<Z> where Z'': "Z'' = Closure\<^sub>\<alpha>\<^sub>,\<^sub>l \<Z>" "A \<turnstile> \<langle>l', Z'\<rangle> \<leadsto> \<langle>l'',\<Z>\<rangle>" by auto
-  from A(2)[OF Z''(2) A(5,6)] obtain Z''' where Z''':
-    "A \<turnstile> \<langle>l, Z\<rangle> \<leadsto>* \<langle>l'',Z'''\<rangle>" "Closure\<^sub>\<alpha>\<^sub>,\<^sub>l \<Z> \<subseteq> Closure\<^sub>\<alpha>\<^sub>,\<^sub>l Z'''"
-  by auto
-  from steps_z_alpha_V[OF A(1,6)] step_z_V[OF Z''(2)] have *: "\<Z> \<subseteq> V" by blast
-  from A Z'' have "A \<turnstile> \<langle>l'', Closure\<^sub>\<alpha>\<^sub>,\<^sub>l \<Z>\<rangle> \<leadsto> \<langle>l''a,Z''a\<rangle>" by auto
-  from calc[OF A(5) * this] obtain \<Z>' where **:
-    "A \<turnstile> \<langle>l'', \<Z>\<rangle> \<leadsto> \<langle>l''a,\<Z>'\<rangle>" "Z''a \<subseteq> Closure\<^sub>\<alpha>\<^sub>,\<^sub>l \<Z>'"
-  by auto
-  from steps_z_alpha_closure_involutive'_aux[OF this(1) Z'''(2) A(5) *] obtain W' where ***:
-    "A \<turnstile> \<langle>l'', Z'''\<rangle> \<leadsto> \<langle>l''a,W'\<rangle>" "Closure\<^sub>\<alpha>\<^sub>,\<^sub>l \<Z>' \<subseteq> Closure\<^sub>\<alpha>\<^sub>,\<^sub>l W'"
-  by auto
-  with Z'''(1) have "A \<turnstile> \<langle>l, Z\<rangle> \<leadsto>* \<langle>l''a,W'\<rangle>" by (blast intro: steps_z_alt)
-  with closure_involutive'[OF **(2)] ***(2) show ?case by blast
-qed
-*)
-
 lemma steps_z_alpha_closure_involutive:
   "A \<turnstile> \<langle>l, Z\<rangle> \<leadsto>\<^sub>\<alpha>* \<langle>l',Z'\<rangle> \<Longrightarrow> valid_abstraction A X k \<Longrightarrow> Z \<subseteq> V
   \<Longrightarrow> \<exists> Z''. A \<turnstile> \<langle>l, Z\<rangle> \<leadsto>* \<langle>l',Z''\<rangle> \<and> Closure\<^sub>\<alpha>\<^sub>,\<^sub>l' Z' \<subseteq> Closure\<^sub>\<alpha>\<^sub>,\<^sub>l' Z'' \<and> Z'' \<subseteq> Z'"
@@ -1343,30 +1006,32 @@ proof (induction A l Z l' Z' rule: steps_z_alpha.induct)
   case refl show ?case by blast
 next
   case 2: (step A l Z l' Z' Z'' a l'' Z''')
-  then obtain Z''a where *: "A \<turnstile> \<langle>l', Z''\<rangle> \<leadsto>\<^bsub>\<upharpoonleft>a\<^esub> \<langle>l'',Z''a\<rangle>" "Z''' = Closure\<^sub>\<alpha>\<^sub>,\<^sub>l'' Z''a" by auto
+  interpret alpha'': AlphaClosure_global _ "k l''" "\<R> l''" by standard (rule finite)
+  have [simp]: \<open>alpha''.cla = cla l''\<close> unfolding alpha''.cla_def cla_def ..
+  from 2 obtain Z''a where *: "A \<turnstile> \<langle>l', Z''\<rangle> \<leadsto>\<^bsub>\<upharpoonleft>a\<^esub> \<langle>l'',Z''a\<rangle>" "Z''' = Closure\<^sub>\<alpha>\<^sub>,\<^sub>l'' Z''a" by auto
   from steps_z_alpha_closure_involutive'[OF 2(1,2) this(1) 2(5,6)] obtain W''' where W''':
     "A \<turnstile> \<langle>l, Z\<rangle> \<leadsto>* \<langle>l'',W'''\<rangle>" "Closure\<^sub>\<alpha>\<^sub>,\<^sub>l'' Z''a \<subseteq> Closure\<^sub>\<alpha>\<^sub>,\<^sub>l'' W'''" "W''' \<subseteq> Z''a" by blast
   have "W''' \<subseteq> Z'''"
-    by (metis "*"(1,2) 2(1,2,6) W'''(3) closure_subs order_trans step_z_V steps_z_alpha_V)
-  with * closure_involutive W''' show ?case by auto
+    by (metis
+        * 2(1,2,6) W'''(3) alpha''.closure_subs[simplified] order_trans step_z_V steps_z_alpha_V
+        )
+  with * alpha''.closure_involutive W''' show ?case by auto
 qed
-
-lemma steps_z_V:
-  "A \<turnstile> \<langle>l, Z\<rangle> \<leadsto>* \<langle>l',Z'\<rangle> \<Longrightarrow> Z \<subseteq> V \<Longrightarrow> Z' \<subseteq> V"
-apply (induction rule: steps_z.induct)
-  apply blast
-using step_z_V by metis
 
 lemma steps_z_alpha_sound:
   "A \<turnstile> \<langle>l, Z\<rangle> \<leadsto>\<^sub>\<alpha>* \<langle>l',Z'\<rangle> \<Longrightarrow> valid_abstraction A X k \<Longrightarrow> Z \<subseteq> V \<Longrightarrow> Z' \<noteq> {}
   \<Longrightarrow> \<exists> Z''. A \<turnstile> \<langle>l, Z\<rangle> \<leadsto>* \<langle>l',Z''\<rangle> \<and> Z'' \<noteq> {} \<and> Z'' \<subseteq> Z'"
 proof goal_cases
   case 1
+  interpret alpha': AlphaClosure_global _ "k l'" "\<R> l'" by standard (rule finite)
+  have [simp]: \<open>alpha'.cla = cla l'\<close> unfolding alpha'.cla_def cla_def ..
   from steps_z_alpha_closure_involutive[OF 1(1-3)] obtain Z'' where
     "A \<turnstile> \<langle>l, Z\<rangle> \<leadsto>* \<langle>l',Z''\<rangle>" "Closure\<^sub>\<alpha>\<^sub>,\<^sub>l' Z' \<subseteq> Closure\<^sub>\<alpha>\<^sub>,\<^sub>l' Z''" "Z'' \<subseteq> Z'"
   by blast
-  moreover with 1(4) cla_empty_iff[OF steps_z_alpha_V[OF 1(1)], OF 1(3)]
-    cla_empty_iff[OF steps_z_V, OF this(1) 1(3)] have "Z'' \<noteq> {}" by auto
+  moreover with
+    1(4) alpha'.cla_empty_iff[OF steps_z_alpha_V[OF 1(1)], OF 1(3)]
+    alpha'.cla_empty_iff[OF steps_z_V, OF this(1) 1(3)]
+  have "Z'' \<noteq> {}" by auto
   ultimately show ?case by auto
 qed
 
